theories/nat_lang/NatLangProperties.v
@@ -1,5 +1,9 @@
 From Triq Require NatLang.
+From Triq Require Import LanguagesCommon.
 From Stdlib Require Import List.
 Import ListNotations.
 
 
+(** Definições de Estado Inicial *)
+Definition is_initial_state (state_nat : NatLang.state) :=
+state_nat Y = 0 /\ forall n, state_nat (Z n) = 0.
