theories/equivalence/StringMacros.v
@@ -1,0 +1,16 @@
+From Triq Require StringLang.
+From Triq Require NatLang.
+
+From Stdlib Require Import List.
+Import ListNotations.
+
+Definition get_str_macro 
+  (i_nat : NatLang.instruction) 
+  (max_char : nat) 
+  (n n' k : nat) 
+  : (StringLang.program) := 
+match i_nat with 
+| NatLang.Instr opt_lbl (NatLang.INCR x) => []
+| NatLang.Instr opt_lbl (NatLang.DECR x) => []
+| NatLang.Instr opt_lbl (NatLang.IF_GOTO x l) => []
+end.
